Write two-column proofs that verify each of the following
logical equivalences.

\begin{enumerate}
\item $A \lor (A \land B) \; \cong \; A \land (A \lor B)$
\medskip

\item $(A \land \lnot B) \lor A \; \cong \; A$
\medskip

\item $A \lor B \; \cong \; A \lor (\lnot A \land B)$
\medskip

\item $\lnot(A \lor \lnot B) \lor (\lnot A \land \lnot B) \; \cong \; \lnot A$
\medskip

\item $A \; \cong \; A \land ((A \lor \lnot B) \lor (A \lor B))$
\medskip

\item $(A \land \lnot B) \land (\lnot A \lor B \; \cong \; c$
\medskip

\item $A \; \cong \; A \land (A \lor (A \land (B \lor C)))$
\medskip

\item $\lnot (A \land B) \land \lnot (A \land C) \; \cong \; \lnot A \lor (\lnot B \land \lnot C)$
\medskip

\end{enumerate}

